\subsection{Statement}
Prove that if the term structure of spot rates is flat, the term structure of
par rates is also flat at the same rate.\par

\subsection{Notaion}
The following notation will be used:\par
\begin{itemize}
    \item
    $T$
    \item
    $r$: Continuous compounding interest rate
\end{itemize}

\subsection{Proof}
\begin{proof}
    \[
        \sum\limits_{t = a}^b{z^t} = z^a + z^{a + 1} + \cdots + z^b
    \]
    \[
        z\sum\limits_{t = a}^b{z^t} = z^{a + 1} + z^{a + 2} + \cdots + z^{b + 1}
    \]
    $\therefore$
    \[
        \begin{array}{ll}
            &z\sum\limits_{t = a}^b{z^t} - \sum\limits_{t = a}^b{z^t}\\
            = &
            z^{b + 1} + (z^b - z^b) + \cdots + (z^{a + 1} - z^{a + 1}) - z^a\\
            = &z^{b + 1} - z^a
        \end{array}
    \]
    $\therefore$
    \[
        \begin{array}{lll}
            (z - 1)\sum\limits_{t = a}^b{z^t} &= &z^{b + 1} - z^a\\
            \sum\limits_{t = a}^b{z^t} &= &
            \frac{z^{b + 1} - z^a}{z - 1}\\
            &= &\frac{z^a - z^{b + 1}}{1 - z}
        \end{array}
    \]
\end{proof}
